commit

AP/System/Symmetry/Defs.lean
@@ -1,191 +1,62 @@
 import AP.System.Invariant
 
-namespace System.Symmetry
+namespace System
 
 universe u
 variable {S T : Type u} {sys : System S T}
 
 @[ext]
-structure Raw (sys : System S T) : Type u where
-  fs : S → S
-  fs' : S → S
-  ft : T → T
-  ft' : T → T
+structure Symmetry (sys : System S T) : Type u where
+  ft : T ≃ T
+  fs : S ≃ S
 
-namespace Raw
+namespace Symmetry
 
-class WF (sym : Raw sys) : Prop where
-  h_fs : ∀ {s}, sys.WF (sym.fs s) ↔ sys.WF s -- derivable?
-  h_fs' : ∀ {s}, sys.WF (sym.fs' s) ↔ sys.WF s -- derivable?
-  h_ft : ∀ {t}, sys.WFTrans (sym.ft t) ↔ sys.WFTrans t -- derivable?
-  h_ft' : ∀ {t}, sys.WFTrans (sym.ft' t) ↔ sys.WFTrans t -- derivable?
-  fs_fs' : Inverse sym.fs sym.fs'
-  ft_ft' : Inverse sym.ft sym.ft'
+def ft' (sym : sys.Symmetry) : T ≃ T := sym.ft.symm
+def fs' (sym : sys.Symmetry) : S ≃ S := sym.fs.symm
+
+class WF (sym : sys.Symmetry) : Prop where
+  initial_fs_iff : ∀ {s}, sys.Initial (sym.fs s) ↔ sys.Initial s
   tr_eq : ∀ {s t}, sys.tr s t = (sys.tr (sym.fs s) (sym.ft t)).map sym.fs'
-  tr_eq' : ∀ {s t}, sys.tr s t = (sys.tr (sym.fs' s) (sym.ft' t)).map sym.fs -- derivable?
 
-def one : Raw sys where
-  fs := id
-  fs' := id
-  ft := id
-  ft' := id
+def one : sys.Symmetry where
+  ft := Equiv.refl T
+  fs := Equiv.refl S
 
-instance : Inhabited (Raw sys) := ⟨one⟩
-theorem default_eq : (default : Raw sys) = one := rfl
+instance : One sys.Symmetry := ⟨one⟩
+theorem one_def : (1 : sys.Symmetry) = one := rfl
+
+instance : Inhabited sys.Symmetry := ⟨1⟩
+theorem default_eq : (default : sys.Symmetry) = 1 := rfl
 
 @[simp]
-def simFn (sym : Raw sys) (f : S → T) (s : S) : T :=
+def simFn (sym : sys.Symmetry) (f : S → T) (s : S) : T :=
   sym.ft # f # sym.fs' s
 
-def inv (sym : Raw sys) : Raw sys where
-  fs := sym.fs'
-  fs' := sym.fs
-  ft' := sym.ft
+def inv (sym : sys.Symmetry) : sys.Symmetry where
   ft := sym.ft'
+  fs := sym.fs'
 
-def mul (sym₁ sym₂ : Raw sys) : Raw sys where
-  fs := sym₁.fs ∘ sym₂.fs
-  fs' := sym₂.fs' ∘ sym₁.fs'
-  ft := sym₁.ft ∘ sym₂.ft
-  ft' := sym₂.ft' ∘ sym₁.ft'
+instance : Inv sys.Symmetry := ⟨inv⟩
+theorem inv_def {sym : sys.Symmetry} : sym⁻¹ = sym.inv := rfl
 
-def div (sym₁ sym₂ : Raw sys) : Raw sys :=
-  sym₁.mul sym₂.inv
+def mul (sym₁ sym₂ : sys.Symmetry) : sys.Symmetry where
+  ft := sym₁.ft.comp sym₂.ft
+  fs := sym₁.fs.comp sym₂.fs
 
-def npow (n : ℕ) (sym : Raw sys) : Raw sys :=
-  (·.mul sym)^[n] one
+instance : Mul sys.Symmetry := ⟨mul⟩
+theorem mul_def {sym₁ sym₂ : sys.Symmetry} : sym₁ * sym₂ = sym₁.mul sym₂ := rfl
 
-def zpow (z : ℤ) (sym : Raw sys) : Raw sys :=
+def div (sym₁ sym₂ : sys.Symmetry) : sys.Symmetry :=
+  sym₁ * sym₂⁻¹
+
+instance : Div sys.Symmetry := ⟨div⟩
+theorem div_def {sym₁ sym₂ : sys.Symmetry} : sym₁ / sym₂ = sym₁ * sym₂⁻¹ := rfl
+
+def npow (n : ℕ) (sym : sys.Symmetry) : sys.Symmetry :=
+  (· * sym)^[n] 1
+
+def zpow (z : ℤ) (sym : sys.Symmetry) : sys.Symmetry :=
   match z with
   | .ofNat n => sym.npow n
-  | .negSucc n => sym.inv.npow (n + 1)
-
------
-
-variable {sym sym₁ sym₂ sym₃ : Raw sys}
-variable [wf : sym.WF] [wf₁ : sym₁.WF] [wf₂ : sym₂.WF] [wf₃ : sym₃.WF]
-
-@[simp] theorem wf_fs_iff {s} : sys.WF (sym.fs s) ↔ sys.WF s := by rw [wf.h_fs]
-@[simp] theorem wf_fs'_iff {s} : sys.WF (sym.fs' s) ↔ sys.WF s := by rw [wf.h_fs']
-@[simp] theorem wf_ft_iff {t} : sys.WFTrans (sym.ft t) ↔ sys.WFTrans t := by rw [wf.h_ft]
-@[simp] theorem wf_ft'_iff {t} : sys.WFTrans (sym.ft' t) ↔ sys.WFTrans t := by rw [wf.h_ft']
-
-instance {s} [hs : sys.WF s] : sys.WF (sym.fs s) := by simpa
-instance {s} [hs : sys.WF s] : sys.WF (sym.fs' s) := by simpa
-instance {t} [ht : sys.WFTrans t] : sys.WFTrans (sym.ft t) := by simpa
-instance {t} [ht : sys.WFTrans t] : sys.WFTrans (sym.ft' t) := by simpa
-
-@[simp] theorem fs_fs' {s} : sym.fs (sym.fs' s) = s := wf.fs_fs'.fg
-@[simp] theorem fs'_fs {s} : sym.fs' (sym.fs s) = s := wf.fs_fs'.gf
-@[simp] theorem ft_ft' {s} : sym.ft (sym.ft' s) = s := wf.ft_ft'.fg
-@[simp] theorem ft'_ft {s} : sym.ft' (sym.ft s) = s := wf.ft_ft'.gf
-
-theorem tr_fs {s t} : sys.tr (sym.fs s) t = (sys.tr s (sym.ft' t)).map sym.fs := by
-  nth_rw 1 [wf.tr_eq']; ext s'; simp
-
-theorem tr_fs' {s t} : sys.tr (sym.fs' s) t = (sys.tr s (sym.ft t)).map sym.fs' := by
-  nth_rw 1 [wf.tr_eq]; ext s'; simp
-
-theorem tr_ft {s t} : sys.tr s (sym.ft t) = (sys.tr (sym.fs' s) t).map sym.fs := by
-  nth_rw 2 [wf.tr_eq]; ext s'; simp
-
-theorem tr_ft' {s t} : sys.tr s (sym.ft' t) = (sys.tr (sym.fs s) t).map sym.fs' := by
-  nth_rw 2 [wf.tr_eq']; ext s'; simp
-
-theorem validTr_fs_of {s t}
-(h : sys.validTr s (sym.ft' t)) : sys.validTr (sym.fs s) t := by
-  obtain ⟨s', h⟩ := h; simp [tr_ft'] at h; obtain ⟨s', h, rfl⟩ := h; use s'
-
-theorem validTr_fs'_of {s t}
-(h : sys.validTr s (sym.ft t)) : sys.validTr (sym.fs' s) t := by
-  obtain ⟨s', h⟩ := h; simp [tr_ft] at h; obtain ⟨s', h, rfl⟩ := h; use s'
-
-theorem validTr_ft_of {s t}
-(h : sys.validTr (sym.fs' s) t) : sys.validTr s (sym.ft t) := by
-  obtain ⟨s', h⟩ := h; simp [tr_fs'] at h; obtain ⟨s', h, rfl⟩ := h; use s'
-
-theorem validTr_ft'_of {s t}
-(h : sys.validTr (sym.fs s) t) : sys.validTr s (sym.ft' t) := by
-  obtain ⟨s', h⟩ := h; simp [tr_fs] at h; obtain ⟨s', h, rfl⟩ := h; use s'
-
-theorem validTr_fs {s t} : sys.validTr (sym.fs s) t ↔ sys.validTr s (sym.ft' t) :=
-  ⟨validTr_ft'_of, validTr_fs_of⟩
-
-theorem validTr_fs' {s t} : sys.validTr (sym.fs' s) t ↔ sys.validTr s (sym.ft t) :=
-  ⟨validTr_ft_of, validTr_fs'_of⟩
-
-theorem validTr_ft {s t} : sys.validTr s (sym.ft t) ↔ sys.validTr (sym.fs' s) t :=
-  ⟨validTr_fs'_of, validTr_ft_of⟩
-
-theorem validTr_ft' {s t} : sys.validTr s (sym.ft' t) ↔ sys.validTr (sym.fs s) t :=
-  ⟨validTr_fs_of, validTr_ft'_of⟩
-
-@[simp]
-theorem hasTr_fs {s} : sys.hasTr (sym.fs s) ↔ sys.hasTr s := by
-  constructor <;> rintro ⟨t, h⟩
-  · use sym.ft' t; simpa [validTr_ft']
-  · use sym.ft t; simpa [validTr_ft]
-
-@[simp]
-theorem hasTr_fs' {s} : sys.hasTr (sym.fs' s) ↔ sys.hasTr s := by
-  constructor <;> rintro ⟨t, h⟩
-  · use sym.ft t; simpa [validTr_ft]
-  · use sym.ft' t; simpa [validTr_ft']
-
-instance : (Raw.one : Raw sys).WF := by
-  unfold Raw.one; constructor <;> simp
-
-instance {f} [hf : sys.SimFn f] : sys.SimFn (sym.simFn f) := by
-  rw [sys.simFn_def]; intro s hs h; simp; apply hf.1 at h; apply validTr_ft_of
-  have h₁ : sys.hasTr (sym.fs' s); simp; exact ⟨_, h⟩; exact hf.1 h₁
-
-instance : sym.inv.WF where
-  h_fs := wf.h_fs'
-  h_fs' := wf.h_fs
-  h_ft := wf.h_ft'
-  h_ft' := wf.h_ft
-  fs_fs' := wf.fs_fs'.symm
-  ft_ft' := wf.ft_ft'.symm
-  tr_eq := wf.tr_eq'
-  tr_eq' := wf.tr_eq
-
-omit wf in @[simp]
-theorem inv_inv : sym.inv.inv = sym := by ext <;> rfl
-
-instance : (sym₁.mul sym₂).WF where
-  h_fs := by simp [mul]
-  h_fs' := by simp [mul]
-  h_ft := by simp [mul]
-  h_ft' := by simp [mul]
-  fs_fs' := by constructor <;> simp [mul]
-  ft_ft' := by constructor <;> simp [mul]
-  tr_eq := by
-    intro s t; ext s'; simp [mul]; constructor
-    · intro h₁; use sym₁.fs # sym₂.fs s'; simp [tr_fs]; use s'
-    · rintro ⟨s', h₁, rfl⟩; simp [tr_ft] at h₁; obtain ⟨s', h₁, rfl⟩ := h₁; simpa
-  tr_eq' := by
-    intro s t; ext s'; simp [mul]; constructor
-    · intro h₁; use sym₂.fs' # sym₁.fs' s'; simp [tr_fs']; use s'
-    · rintro ⟨s', h₁, rfl⟩; simp [tr_ft'] at h₁; obtain ⟨s', h₁, rfl⟩ := h₁; simpa
-
-instance : (sym₁.div sym₂).WF := by
-  unfold div; infer_instance
-
-instance {n} : (sym.npow n).WF := by
-  simp [npow]; induction n; simp; infer_instance; nm n ih
-  rw [Function.iterate_succ']; simp; infer_instance
-
-instance {z} : (sym.zpow z).WF := by
-  simp [zpow]; split <;> infer_instance
-
-@[simp]
-protected theorem inv_mul_cancel : sym.inv.mul sym = one := by
-  simp [inv, mul, one]; constructor <;> ext <;> simp
-
-omit wf₁ @[simp]
-protected theorem inv_eq_of_mul (h : sym₁.mul sym₂ = one) : sym₁.inv = sym₂ := by
-  simp [inv, mul, one] at h ⊢; rcases h with ⟨h₁, h₂, h₃, h₄⟩; ext <;> dsimp
-  · nm s; apply congrArg sym₂.fs ∘ congrArg (· s) at h₂; simp at h₂; exact h₂
-  · nm s; apply congrArg (· # sym₂.fs' s) at h₁; simp at h₁; exact h₁
-  · nm t; apply congrArg sym₂.ft ∘ congrArg (· t) at h₄; simp at h₄; exact h₄
-  · nm t; apply congrArg (· # sym₂.ft' t) at h₃; simp at h₃; exact h₃
+  | .negSucc n => sym⁻¹.npow (n + 1)
